Add world to HeapLang

nola/examples/heap_lang/primitive_laws.v
@@ -11,20 +11,22 @@ From nola.examples.heap_lang Require Export class_instances.
 From nola.examples.heap_lang Require Import tactics notation.
 From iris.prelude Require Import options.
 
-Class heapGS_gen hlc Σ := HeapGS {
+(** We introduce the world parameter [W] *)
+Class heapGS_gen hlc Σ (X : Type) (W : X → iProp Σ) := HeapGS {
   heapGS_invGS : invGS_gen hlc Σ;
   heapGS_gen_heapGS :: gen_heapGS loc (option val) Σ;
   heapGS_inv_heapGS :: inv_heapGS loc (option val) Σ;
   heapGS_proph_mapGS :: proph_mapGS proph_id (val * val) Σ;
   heapGS_step_name : gname;
   heapGS_step_cnt : mono_natG Σ;
+  heapGS_wolrd_arg : X;
 }.
 Local Existing Instance heapGS_step_cnt.
 
 Notation heapGS := (heapGS_gen HasLc).
 
 Section steps.
-  Context `{!heapGS_gen hlc Σ}.
+  Context `{!heapGS_gen hlc Σ X W}.
 
   Local Definition steps_auth (n : nat) : iProp Σ :=
     mono_nat_auth_own heapGS_step_name 1 n.
@@ -60,16 +62,16 @@ Section steps.
 
 End steps.
 
-Global Program Instance heapGS_irisGS `{!heapGS_gen hlc Σ} : irisGS_gen hlc heap_ectxi_lang Σ := {
+Global Program Instance heapGS_irisGS `{!heapGS_gen hlc Σ X W} : irisGS_gen hlc heap_ectxi_lang Σ := {
   iris_invGS := heapGS_invGS;
   state_interp σ step_cnt κs _ :=
-    (gen_heap_interp σ.(heap) ∗ proph_map_interp κs σ.(used_proph_id) ∗
+    (W heapGS_wolrd_arg ∗ gen_heap_interp σ.(heap) ∗ proph_map_interp κs σ.(used_proph_id) ∗
      steps_auth step_cnt)%I;
   fork_post _ := True%I;
   num_laters_per_step n := n;
 }.
 Next Obligation.
-  iIntros (??? σ ns κs nt)  "/= ($ & $ & H)".
+  iIntros (????? σ ns κs nt) "/= ($ & $ & $ & H)".
   by iMod (steps_auth_update_S with "H") as "$".
 Qed.
 
@@ -82,7 +84,7 @@ Notation "l ↦ dq v" := (mapsto (L:=loc) (V:=option val) l dq (Some v%V))
 make setoid rewriting in the predicate [I] work we need actual definitions
 here. *)
 Section definitions.
-  Context `{!heapGS_gen hlc Σ}.
+  Context `{!heapGS_gen hlc Σ X W}.
   Definition inv_mapsto_own (l : loc) (v : val) (I : val → Prop) : iProp Σ :=
     inv_mapsto_own l (Some v) (from_option I False).
   Definition inv_mapsto (l : loc) (I : val → Prop) : iProp Σ :=
@@ -99,7 +101,7 @@ Notation "l ↦_ I v" := (inv_mapsto_own l v I%stdpp%type)
   (at level 20, I at level 9, format "l  ↦_ I  v") : bi_scope.
 
 Section lifting.
-Context `{!heapGS_gen hlc Σ}.
+Context `{!heapGS_gen hlc Σ X W}.
 Implicit Types P Q : iProp Σ.
 Implicit Types Φ Ψ : val → iProp Σ.
 Implicit Types efs : list expr.
@@ -115,7 +117,7 @@ Proof.
   (** TODO: We should try to use a generic lifting lemma (and avoid [wp_unfold])
   here, since this breaks the WP abstraction. *)
   rewrite !wp_unfold /wp_pre /=. iIntros (->) "Hwp".
-  iIntros (σ1 ns κ κs m) "(Hσ & Hκ & Hsteps)".
+  iIntros (σ1 ns κ κs m) "(W & Hσ & Hκ & Hsteps)".
   iDestruct (steps_lb_get with "Hsteps") as "#Hlb".
   iDestruct (steps_lb_le _ 0 with "Hlb") as "Hlb0"; [lia|].
   iSpecialize ("Hwp" with "Hlb0"). iApply ("Hwp" $! σ1 ns κ κs m). iFrame.
@@ -130,15 +132,15 @@ Proof.
   (** TODO: We should try to use a generic lifting lemma (and avoid [wp_unfold])
   here, since this breaks the WP abstraction. *)
   rewrite !wp_unfold /wp_pre /=. iIntros (->) "Hlb Hwp".
-  iIntros (σ1 ns κ κs m) "(Hσ & Hκ & Hsteps)".
+  iIntros (σ1 ns κ κs m) "(W & Hσ & Hκ & Hsteps)".
   iDestruct (steps_lb_valid with "Hsteps Hlb") as %?.
-  iMod ("Hwp" $! σ1 ns κ κs m with "[$Hσ $Hκ $Hsteps]") as "[%Hs Hwp]".
+  iMod ("Hwp" $! σ1 ns κ κs m with "[$W $Hσ $Hκ $Hsteps]") as "[%Hs Hwp]".
   iModIntro. iSplit; [done|].
   iIntros (e2 σ2 efs Hstep) "Hcred".
   iMod ("Hwp" with "[//] Hcred") as "Hwp".
   iIntros "!> !>". iMod "Hwp" as "Hwp". iIntros "!>".
   iApply (step_fupdN_wand with "Hwp").
-  iIntros "Hwp". iMod "Hwp" as "(($ & $ & Hsteps)& Hwp & $)".
+  iIntros "Hwp". iMod "Hwp" as "(($ & $ & $ & Hsteps)& Hwp & $)".
   iDestruct (steps_lb_get with "Hsteps") as "#HlbS".
   iDestruct (steps_lb_le _ (S n) with "HlbS") as "#HlbS'"; [lia|].
   iModIntro. iFrame "Hsteps".
@@ -156,7 +158,7 @@ Proof.
   iIntros (He HE) "Hlb HP Hwp".
   iApply wp_step_fupdN; [done|].
   iSplit; [|by iFrame].
-  iIntros (σ ns κs nt) "(? & ? & Hsteps)".
+  iIntros (σ ns κs nt) "(? & ? & ? & Hsteps)".
   iDestruct (steps_lb_valid with "Hsteps Hlb") as %Hle.
   iApply fupd_mask_intro; [set_solver|].
   iIntros "_". iPureIntro. rewrite /num_laters_per_step /=. lia.
@@ -181,7 +183,7 @@ Lemma wp_fork s E e Φ :
   ▷ WP e @ s; ⊤ {{ _, True }} -∗ ▷ Φ (LitV LitUnit) -∗ WP Fork e @ s; E {{ Φ }}.
 Proof.
   iIntros "He HΦ". iApply wp_lift_atomic_head_step; [done|].
-  iIntros (σ1 ns κ κs nt) "(?&?&Hsteps) !>"; iSplit; first by eauto with head_step.
+  iIntros (σ1 ns κ κs nt) "(?&?&?&Hsteps) !>"; iSplit; first by eauto with head_step.
   iIntros "!>" (v2 σ2 efs Hstep) "_"; inv_head_step.
   iMod (steps_auth_update_S with "Hsteps") as "Hsteps".
   by iFrame.
@@ -191,7 +193,7 @@ Lemma twp_fork s E e Φ :
   WP e @ s; ⊤ [{ _, True }] -∗ Φ (LitV LitUnit) -∗ WP Fork e @ s; E [{ Φ }].
 Proof.
   iIntros "He HΦ". iApply twp_lift_atomic_head_step; [done|].
-  iIntros (σ1 ns κs nt) "(?&?&Hsteps) !>"; iSplit; first by eauto with head_step.
+  iIntros (σ1 ns κs nt) "(?&?&?&Hsteps) !>"; iSplit; first by eauto with head_step.
   iIntros (κ v2 σ2 efs Hstep); inv_head_step.
   iMod (steps_auth_update_S with "Hsteps") as "Hsteps".
   by iFrame.
@@ -328,14 +330,14 @@ Lemma twp_allocN_seq s E v n :
       (l +ₗ (i : nat)) ↦ v ∗ meta_token (l +ₗ (i : nat)) ⊤ }]].
 Proof.
   iIntros (Hn Φ) "_ HΦ". iApply twp_lift_atomic_head_step_no_fork; first done.
-  iIntros (σ1 ns κs nt) "(Hσ & Hκs & Hsteps) !>"; iSplit; first by destruct n; auto with lia head_step.
+  iIntros (σ1 ns κs nt) "(W & Hσ & Hκs & Hsteps) !>"; iSplit; first by destruct n; auto with lia head_step.
   iIntros (κ v2 σ2 efs Hstep); inv_head_step.
   iMod (gen_heap_alloc_big _ (heap_array _ (replicate (Z.to_nat n) v)) with "Hσ")
     as "(Hσ & Hl & Hm)".
   { apply heap_array_map_disjoint.
     rewrite replicate_length Z2Nat.id; auto with lia. }
   iMod (steps_auth_update_S with "Hsteps") as "Hsteps".
-  iModIntro; do 2 (iSplit; first done). iFrame "Hσ Hκs Hsteps". iApply "HΦ".
+  iModIntro; do 2 (iSplit; first done). iFrame "W Hσ Hκs Hsteps". iApply "HΦ".
   iApply big_sepL_sep. iSplitL "Hl".
   - by iApply heap_array_to_seq_mapsto.
   - iApply (heap_array_to_seq_meta with "Hm"). by rewrite replicate_length.
@@ -368,7 +370,7 @@ Lemma twp_free s E l v :
   [[{ RET LitV LitUnit; True }]].
 Proof.
   iIntros (Φ) "Hl HΦ". iApply twp_lift_atomic_head_step_no_fork; first done.
-  iIntros (σ1 ns κs nt) "(Hσ & Hκs & Hsteps) !>". iDestruct (gen_heap_valid with "Hσ Hl") as %?.
+  iIntros (σ1 ns κs nt) "(W & Hσ & Hκs & Hsteps) !>". iDestruct (gen_heap_valid with "Hσ Hl") as %?.
   iSplit; first by eauto with head_step.
   iIntros (κ v2 σ2 efs Hstep); inv_head_step.
   iMod (gen_heap_update with "Hσ Hl") as "[$ Hl]".
@@ -387,7 +389,7 @@ Lemma twp_load s E l dq v :
   [[{ l ↦{dq} v }]] Load (Val $ LitV $ LitLoc l) @ s; E [[{ RET v; l ↦{dq} v }]].
 Proof.
   iIntros (Φ) "Hl HΦ". iApply twp_lift_atomic_head_step_no_fork; first done.
-  iIntros (σ1 ns κs nt) "(Hσ & Hκs & Hsteps) !>". iDestruct (gen_heap_valid with "Hσ Hl") as %?.
+  iIntros (σ1 ns κs nt) "(W & Hσ & Hκs & Hsteps) !>". iDestruct (gen_heap_valid with "Hσ Hl") as %?.
   iSplit; first by eauto with head_step.
   iIntros (κ v2 σ2 efs Hstep); inv_head_step.
   iMod (steps_auth_update_S with "Hsteps") as "Hsteps".
@@ -406,7 +408,7 @@ Lemma twp_store s E l v' v :
   [[{ RET LitV LitUnit; l ↦ v }]].
 Proof.
   iIntros (Φ) "Hl HΦ". iApply twp_lift_atomic_head_step_no_fork; first done.
-  iIntros (σ1 ns κs nt) "(Hσ & Hκs & Hsteps) !>". iDestruct (gen_heap_valid with "Hσ Hl") as %?.
+  iIntros (σ1 ns κs nt) "(W & Hσ & Hκs & Hsteps) !>". iDestruct (gen_heap_valid with "Hσ Hl") as %?.
   iSplit; first by eauto with head_step.
   iIntros (κ v2 σ2 efs Hstep); inv_head_step.
   iMod (steps_auth_update_S with "Hsteps") as "Hsteps".
@@ -426,7 +428,7 @@ Lemma twp_xchg s E l v' v :
   [[{ RET v'; l ↦ v }]].
 Proof.
   iIntros (Φ) "Hl HΦ". iApply twp_lift_atomic_head_step_no_fork; first done.
-  iIntros (σ1 ns κs nt) "(Hσ & Hκs & Hsteps) !>". iDestruct (gen_heap_valid with "Hσ Hl") as %?.
+  iIntros (σ1 ns κs nt) "(W & Hσ & Hκs & Hsteps) !>". iDestruct (gen_heap_valid with "Hσ Hl") as %?.
   iSplit; first by eauto with head_step.
   iIntros (κ v2 σ2 efs Hstep); inv_head_step.
   iMod (steps_auth_update_S with "Hsteps") as "Hsteps".
@@ -447,7 +449,7 @@ Lemma twp_cmpxchg_fail s E l dq v' v1 v2 :
   [[{ RET PairV v' (LitV $ LitBool false); l ↦{dq} v' }]].
 Proof.
   iIntros (?? Φ) "Hl HΦ". iApply twp_lift_atomic_head_step_no_fork; first done.
-  iIntros (σ1 ns κs nt) "(Hσ & Hκs & Hsteps) !>". iDestruct (gen_heap_valid with "Hσ Hl") as %?.
+  iIntros (σ1 ns κs nt) "(W & Hσ & Hκs & Hsteps) !>". iDestruct (gen_heap_valid with "Hσ Hl") as %?.
   iSplit; first by eauto with head_step.
   iIntros (κ v2' σ2 efs Hstep); inv_head_step.
   rewrite bool_decide_false //.
@@ -469,7 +471,7 @@ Lemma twp_cmpxchg_suc s E l v1 v2 v' :
   [[{ RET PairV v' (LitV $ LitBool true); l ↦ v2 }]].
 Proof.
   iIntros (?? Φ) "Hl HΦ". iApply twp_lift_atomic_head_step_no_fork; first done.
-  iIntros (σ1 ns κs nt) "(Hσ & Hκs & Hsteps) !>". iDestruct (gen_heap_valid with "Hσ Hl") as %?.
+  iIntros (σ1 ns κs nt) "(W & Hσ & Hκs & Hsteps) !>". iDestruct (gen_heap_valid with "Hσ Hl") as %?.
   iSplit; first by eauto with head_step.
   iIntros (κ v2' σ2 efs Hstep); inv_head_step.
   rewrite bool_decide_true //.
@@ -491,7 +493,7 @@ Lemma twp_faa s E l i1 i2 :
   [[{ RET LitV (LitInt i1); l ↦ LitV (LitInt (i1 + i2)) }]].
 Proof.
   iIntros (Φ) "Hl HΦ". iApply twp_lift_atomic_head_step_no_fork; first done.
-  iIntros (σ1 ns κs nt) "(Hσ & Hκs & Hsteps) !>". iDestruct (gen_heap_valid with "Hσ Hl") as %?.
+  iIntros (σ1 ns κs nt) "(W & Hσ & Hκs & Hsteps) !>". iDestruct (gen_heap_valid with "Hσ Hl") as %?.
   iSplit; first by eauto with head_step.
   iIntros (κ e2 σ2 efs Hstep); inv_head_step.
   iMod (gen_heap_update with "Hσ Hl") as "[$ Hl]".
@@ -512,7 +514,7 @@ Lemma wp_new_proph s E :
   {{{ pvs p, RET (LitV (LitProphecy p)); proph p pvs }}}.
 Proof.
   iIntros (Φ) "_ HΦ". iApply wp_lift_atomic_head_step_no_fork; first done.
-  iIntros (σ1 ns κ κs nt) "(Hσ & HR & Hsteps) !>". iSplit; first by eauto with head_step.
+  iIntros (σ1 ns κ κs nt) "(W & Hσ & HR & Hsteps) !>". iSplit; first by eauto with head_step.
   iIntros "!>" (v2 σ2 efs Hstep) "_". inv_head_step.
   rename select proph_id into p.
   iMod (steps_auth_update_S with "Hsteps") as "Hsteps".
@@ -572,22 +574,22 @@ Proof.
   (* TODO we should try to use a generic lifting lemma (and avoid [wp_unfold])
      here, since this breaks the WP abstraction. *)
   iIntros (A He) "Hp WPe". rewrite !wp_unfold /wp_pre /= He. simpl in *.
-  iIntros (σ1 ns κ κs nt) "(Hσ & Hκ & Hsteps)".
+  iIntros (σ1 ns κ κs nt) "(W & Hσ & Hκ & Hsteps)".
   destruct κ as [|[p' [w' v']] κ' _] using rev_ind.
-  - iMod ("WPe" $! σ1 ns [] κs nt with "[$Hσ $Hκ $Hsteps]") as "[Hs WPe]".
+  - iMod ("WPe" $! σ1 ns [] κs nt with "[$W $Hσ $Hκ $Hsteps]") as "[Hs WPe]".
     iModIntro. iSplit.
     { iDestruct "Hs" as "%". iPureIntro. destruct s; [ by apply resolve_reducible | done]. }
     iIntros (e2 σ2 efs step). exfalso. apply step_resolve in step; last done.
     inv_head_step. match goal with H: ?κs ++ [_] = [] |- _ => by destruct κs end.
   - rewrite -assoc.
-    iMod ("WPe" $! σ1 ns _ _ nt with "[$Hσ $Hκ $Hsteps]") as "[Hs WPe]". iModIntro. iSplit.
+    iMod ("WPe" $! σ1 ns _ _ nt with "[$W $Hσ $Hκ $Hsteps]") as "[Hs WPe]". iModIntro. iSplit.
     { iDestruct "Hs" as %?. iPureIntro. destruct s; [ by apply resolve_reducible | done]. }
     iIntros (e2 σ2 efs step) "Hcred". apply step_resolve in step; last done.
     inv_head_step; simplify_list_eq.
     iMod ("WPe" $! (Val w') σ2 efs with "[%] Hcred") as "WPe".
     { by eexists [] _ _. }
     iModIntro. iNext. iMod "WPe" as "WPe". iModIntro.
-    iApply (step_fupdN_wand with "WPe"); iIntros "> [($ & Hκ & $) WPe]".
+    iApply (step_fupdN_wand with "WPe"); iIntros "> [($ & $ & Hκ & $) WPe]".
     iMod (proph_map_resolve_proph p' (w',v') κs with "[$Hκ $Hp]") as (vs' ->) "[$ HPost]".
     iModIntro. rewrite !wp_unfold /wp_pre /=. iDestruct "WPe" as "[HΦ $]".
     iMod "HΦ". iModIntro. by iApply "HΦ".
@@ -597,7 +599,7 @@ Lemma twp_ndnat s E :
   [[{ True }]] Ndnat @ s; E [[{ (n : nat), RET (LitV (LitInt n)); True }]].
 Proof.
   iIntros (Φ) "_ HΦ". iApply twp_lift_atomic_head_step_no_fork; first done.
-  iIntros (σ1 ns κs nt) "(Hσ & Hκs & Hsteps) !>".
+  iIntros (σ1 ns κs nt) "(W & Hσ & Hκs & Hsteps) !>".
   iSplit; [by auto with head_step|]. iIntros (κ v2 σ2 efs Hstep); inv_head_step.
   iMod (steps_auth_update_S with "Hsteps") as "Hsteps".
   iModIntro. do 2 (iSplit; [done|]). iFrame. by iApply "HΦ".
