nola/examples/heap_lang/proofmode.v
@@ -6,11 +6,11 @@ From nola.examples.heap_lang Require Import notation.
 From iris.prelude Require Import options.
 Import uPred.
 
-Lemma tac_wp_expr_eval `{!heapGS_gen hlc Σ} Δ s E Φ e e' :
+Lemma tac_wp_expr_eval `{!heapGS_gen hlc Σ X W} Δ s E Φ e e' :
   (∀ (e'':=e'), e = e'') →
   envs_entails Δ (WP e' @ s; E {{ Φ }}) → envs_entails Δ (WP e @ s; E {{ Φ }}).
 Proof. by intros ->. Qed.
-Lemma tac_twp_expr_eval `{!heapGS_gen hlc Σ} Δ s E Φ e e' :
+Lemma tac_twp_expr_eval `{!heapGS_gen hlc Σ X W} Δ s E Φ e e' :
   (∀ (e'':=e'), e = e'') →
   envs_entails Δ (WP e' @ s; E [{ Φ }]) → envs_entails Δ (WP e @ s; E [{ Φ }]).
 Proof. by intros ->. Qed.
@@ -28,7 +28,7 @@ Tactic Notation "wp_expr_eval" tactic3(t) :=
   end.
 Ltac wp_expr_simpl := wp_expr_eval simpl.
 
-Lemma tac_wp_pure `{!heapGS_gen hlc Σ} Δ Δ' s E K e1 e2 φ n Φ :
+Lemma tac_wp_pure `{!heapGS_gen hlc Σ X W} Δ Δ' s E K e1 e2 φ n Φ :
   PureExec φ n e1 e2 →
   φ →
   MaybeIntoLaterNEnvs n Δ Δ' →
@@ -41,7 +41,7 @@ Proof.
   rewrite HΔ' -lifting.wp_pure_step_later //.
   iIntros "Hwp !> _" => //.
 Qed.
-Lemma tac_twp_pure `{!heapGS_gen hlc Σ} Δ s E K e1 e2 φ n Φ :
+Lemma tac_twp_pure `{!heapGS_gen hlc Σ X W} Δ s E K e1 e2 φ n Φ :
   PureExec φ n e1 e2 →
   φ →
   envs_entails Δ (WP (fill K e2) @ s; E [{ Φ }]) →
@@ -53,7 +53,7 @@ Proof.
   rewrite -total_lifting.twp_pure_step //.
 Qed.
 
-Lemma tac_wp_pure_credit `{!heapGS_gen hlc Σ} Δ Δ' s E j K e1 e2 ϕ Φ :
+Lemma tac_wp_pure_credit `{!heapGS_gen hlc Σ X W} Δ Δ' s E j K e1 e2 ϕ Φ :
   PureExec ϕ 1 e1 e2 →
   ϕ →
   MaybeIntoLaterNEnvs 1 Δ Δ' →
@@ -73,17 +73,17 @@ Proof.
   rewrite right_id. apply wand_intro_r. by rewrite wand_elim_l.
 Qed.
 
-Lemma tac_wp_value_nofupd `{!heapGS_gen hlc Σ} Δ s E Φ v :
+Lemma tac_wp_value_nofupd `{!heapGS_gen hlc Σ X W} Δ s E Φ v :
   envs_entails Δ (Φ v) → envs_entails Δ (WP (Val v) @ s; E {{ Φ }}).
 Proof. rewrite envs_entails_unseal=> ->. by apply wp_value. Qed.
-Lemma tac_twp_value_nofupd `{!heapGS_gen hlc Σ} Δ s E Φ v :
+Lemma tac_twp_value_nofupd `{!heapGS_gen hlc Σ X W} Δ s E Φ v :
   envs_entails Δ (Φ v) → envs_entails Δ (WP (Val v) @ s; E [{ Φ }]).
 Proof. rewrite envs_entails_unseal=> ->. by apply twp_value. Qed.
 
-Lemma tac_wp_value `{!heapGS_gen hlc Σ} Δ s E (Φ : val → iPropI Σ) v :
+Lemma tac_wp_value `{!heapGS_gen hlc Σ X W} Δ s E (Φ : val → iPropI Σ) v :
   envs_entails Δ (|={E}=> Φ v) → envs_entails Δ (WP (Val v) @ s; E {{ Φ }}).
 Proof. rewrite envs_entails_unseal=> ->. by rewrite wp_value_fupd. Qed.
-Lemma tac_twp_value `{!heapGS_gen hlc Σ} Δ s E (Φ : val → iPropI Σ) v :
+Lemma tac_twp_value `{!heapGS_gen hlc Σ X W} Δ s E (Φ : val → iPropI Σ) v :
   envs_entails Δ (|={E}=> Φ v) → envs_entails Δ (WP (Val v) @ s; E [{ Φ }]).
 Proof. rewrite envs_entails_unseal=> ->. by rewrite twp_value_fupd. Qed.
 
@@ -221,12 +221,12 @@ Tactic Notation "wp_inj" := wp_pure (InjL _) || wp_pure (InjR _).
 Tactic Notation "wp_pair" := wp_pure (Pair _ _).
 Tactic Notation "wp_closure" := wp_pure (Rec _ _ _).
 
-Lemma tac_wp_bind `{!heapGS_gen hlc Σ} K Δ s E Φ e f :
+Lemma tac_wp_bind `{!heapGS_gen hlc Σ X W} K Δ s E Φ e f :
   f = (λ e, fill K e) → (* as an eta expanded hypothesis so that we can `simpl` it *)
   envs_entails Δ (WP e @ s; E {{ v, WP f (Val v) @ s; E {{ Φ }} }})%I →
   envs_entails Δ (WP fill K e @ s; E {{ Φ }}).
 Proof. rewrite envs_entails_unseal=> -> ->. by apply: wp_bind. Qed.
-Lemma tac_twp_bind `{!heapGS_gen hlc Σ} K Δ s E Φ e f :
+Lemma tac_twp_bind `{!heapGS_gen hlc Σ X W} K Δ s E Φ e f :
   f = (λ e, fill K e) → (* as an eta expanded hypothesis so that we can `simpl` it *)
   envs_entails Δ (WP e @ s; E [{ v, WP f (Val v) @ s; E [{ Φ }] }])%I →
   envs_entails Δ (WP fill K e @ s; E [{ Φ }]).
@@ -257,7 +257,7 @@ Tactic Notation "wp_bind" open_constr(efoc) :=
 
 (** Heap tactics *)
 Section heap.
-Context `{!heapGS_gen hlc Σ}.
+Context `{!heapGS_gen hlc Σ X W}.
 Implicit Types P Q : iProp Σ.
 Implicit Types Φ : val → iProp Σ.
 Implicit Types Δ : envs (uPredI (iResUR Σ)).
